README.md
@@ -1,2 +1,4 @@
 # Formal Verification of the LZ77 Compression Algorithm
 
+[VCT manual](https://github.com/PrincetonUniversity/VST/blob/master/doc/VC.pdf)
+
